thy/Primitive_Matchers/Code_Interface.thy
@@ -73,8 +73,8 @@ text\<open>Example\<close>
 context
 begin
   (*cool example*)
-  lemma "let fw = [''FORWARD'' \<mapsto> [Rule (Match (Src (Ip4AddrNetmask (10,0,0,0) 8))) (Call ''foo'')],
-                   ''foo'' \<mapsto> [Rule (Match (Src (Ip4AddrNetmask (10,128,0,0) 9))) action.Return,
+  lemma "let fw = [''FORWARD'' \<mapsto> [Rule (Match (Src (IpAddrNetmask (ipv4addr_of_dotdecimal (10,0,0,0)) 8))) (Call ''foo'')],
+                   ''foo'' \<mapsto> [Rule (Match (Src (IpAddrNetmask (ipv4addr_of_dotdecimal (10,128,0,0)) 9))) action.Return,
                                Rule (Match (Prot (Proto TCP))) action.Accept]
                    ] in
     let simplfw = to_simple_firewall
@@ -86,8 +86,8 @@ begin
   
   (*cooler example*)
   private definition "cool_example \<equiv> (let fw = 
-                [''FORWARD'' \<mapsto> [Rule (Match (Src (Ip4AddrNetmask (10,0,0,0) 8))) (Call ''foo'')],
-                 ''foo'' \<mapsto> [Rule (MatchNot (Match (Src (Ip4AddrNetmask (10,0,0,0) 9)))) action.Drop,
+                [''FORWARD'' \<mapsto> [Rule (Match (Src (IpAddrNetmask (ipv4addr_of_dotdecimal (10,0,0,0)) 8))) (Call ''foo'')],
+                 ''foo'' \<mapsto> [Rule (MatchNot (Match (Src (IpAddrNetmask (ipv4addr_of_dotdecimal (10,0,0,0)) 9)))) action.Drop,
                              Rule (Match (Prot (Proto TCP))) action.Accept]
                  ] in
     to_simple_firewall (upper_closure (optimize_matches abstract_for_simple_firewall
@@ -120,9 +120,9 @@ context
 begin
   (*now with a destination IP*)
   private definition "cool_example2 \<equiv> (let fw =
-    [''FORWARD'' \<mapsto> [Rule (Match (Src (Ip4AddrNetmask (10,0,0,0) 8))) (Call ''foo'')],
-     ''foo'' \<mapsto> [Rule (MatchNot (Match (Src (Ip4AddrNetmask (10,0,0,0) 9)))) action.Drop,
-                 Rule (MatchAnd (Match (Prot (Proto TCP))) (Match (Dst (Ip4AddrNetmask (10,0,0,42) 32)))) action.Accept]
+    [''FORWARD'' \<mapsto> [Rule (Match (Src (IpAddrNetmask (ipv4addr_of_dotdecimal (10,0,0,0)) 8))) (Call ''foo'')],
+     ''foo'' \<mapsto> [Rule (MatchNot (Match (Src (IpAddrNetmask (ipv4addr_of_dotdecimal (10,0,0,0)) 9)))) action.Drop,
+                 Rule (MatchAnd (Match (Prot (Proto TCP))) (Match (Dst (IpAddrNetmask (ipv4addr_of_dotdecimal (10,0,0,42)) 32)))) action.Accept]
                 ] in
     to_simple_firewall (upper_closure (optimize_matches abstract_for_simple_firewall
                           (upper_closure (packet_assume_new (unfold_ruleset_FORWARD action.Drop fw))))))"
